added NTM and ISMin_intro

Term/WithArity/AInfSeq.v
@@ -11,7 +11,7 @@ WF_absorb. *)
 Set Implicit Arguments.
 
 Require Import RelUtil ATrs LogicUtil ACalls SN InfSeq NatLeast List
-  IndefiniteDescription.
+  IndefiniteDescription ClassicalChoice ProofIrrelevance.
 
 Section S.
 
@@ -20,48 +20,6 @@ Section S.
   Notation term := (term Sig).
   Notation subterm_eq := (@subterm_eq Sig).
   Notation supterm_eq := (@supterm_eq Sig).
-
-(*****************************************************************************)
-(** minimal non-terminating subterm *)
-
-  Section NT_min.
-
-    Variables (R : relation term) (t : term) (ht : NT R t).
-
-    Lemma NT_min_intro : exists u, subterm_eq u t /\ NT_min R u.
-
-    Proof.
-      set (P := fun n => exists u, subterm_eq u t /\ size u = n /\ NT R u).
-      assert (exP : exists n, P n). exists (size t). exists t. split.
-      apply subterm_eq_refl. intuition.
-      destruct (ch_min P exP) as [n [[Pn nleP] nmin]].
-      destruct Pn as [u [ut [un hu]]]. subst n. exists u. unfold NT_min.
-      intuition. rename u0 into v.
-      assert (size u <= size v). apply nleP. exists v. intuition.
-      eapply subterm_eq_trans. apply subterm_strict. apply H. hyp.
-      ded (subterm_size H). omega.
-    Qed.
-
-    Definition min_term :=
-      projT1 (constructive_indefinite_description _ NT_min_intro).
-
-    Lemma NT_min_term : NT_min R min_term.
-
-    Proof.
-      unfold min_term. destruct (constructive_indefinite_description
-      (fun u : term => subterm_eq u t /\ NT_min R u) NT_min_intro) as [u hu].
-      simpl. intuition.
-    Qed.
-
-    Lemma subterm_min_term : subterm_eq min_term t.
-
-    Proof.
-      unfold min_term. destruct (constructive_indefinite_description
-      (fun u : term => subterm_eq u t /\ NT_min R u) NT_min_intro) as [u hu].
-      simpl. intuition.
-    Qed.
-
-  End NT_min.
 
 (*****************************************************************************)
 (** general boolean conditions for which [WF (hd_red_mod R D)] is
@@ -114,5 +72,98 @@ equivalent to [WF (hd_red_Mod (int_red R #) D)] *)
     Qed.
 
   End WF_hd_red_mod_from_WF_hd_red_Mod_int.
+
+(*****************************************************************************)
+(** subtype of minimal non-terminating terms *)
+
+  Section NTM.
+
+    Variable R : relation term.
+
+    Record NTM : Type := mkNTM {
+      NTM_val :> term;
+      NTM_prop :> NT_min R NTM_val }.
+
+  End NTM.
+
+(*****************************************************************************)
+(** getting a minimal non-terminating subterm *)
+
+  Section NT_min.
+
+    Variables (R : relation term) (t : term) (ht : NT R t).
+
+    Lemma NT_min_intro : exists u, subterm_eq u t /\ NT_min R u.
+
+    Proof.
+      set (P := fun n => exists u, subterm_eq u t /\ size u = n /\ NT R u).
+      assert (exP : exists n, P n). exists (size t). exists t. split.
+      apply subterm_eq_refl. intuition.
+      destruct (ch_min P exP) as [n [[Pn nleP] nmin]].
+      destruct Pn as [u [ut [un hu]]]. subst n. exists u. unfold NT_min, min.
+      intuition. rename u0 into v.
+      assert (size u <= size v). apply nleP. exists v. intuition.
+      eapply subterm_eq_trans. apply subterm_strict. apply H. hyp.
+      ded (subterm_size H). omega.
+    Qed.
+
+    Definition min_term :=
+      projT1 (constructive_indefinite_description _ NT_min_intro).
+
+    Lemma NT_min_term : NT_min R min_term.
+
+    Proof.
+      unfold min_term. destruct (constructive_indefinite_description
+      (fun u : term => subterm_eq u t /\ NT_min R u) NT_min_intro) as [u hu].
+      simpl. intuition.
+    Qed.
+
+    Lemma subterm_eq_min_term : subterm_eq min_term t.
+
+    Proof.
+      unfold min_term. destruct (constructive_indefinite_description
+      (fun u : term => subterm_eq u t /\ NT_min R u) NT_min_intro) as [u hu].
+      simpl. intuition.
+    Qed.
+
+  End NT_min.
+
+(*****************************************************************************)
+(** getting a minimal infinite (R @ supterm_eq)-sequence from an
+infinite R-sequence *)
+
+  Section ISMin.
+
+    Variable R : relation term.
+
+    Definition S : relation (NTM R) := R @ supterm_eq.
+
+    Lemma S_left_total : forall t, exists u, S t u.
+
+    Proof.
+      intros [t [[f [h0 hf]] ht]].
+      exists (mkNTM (NT_min_term (NT_IS_elt 1 hf))).
+      unfold S. simpl. exists (f 1). subst t. intuition.
+      apply subterm_eq_min_term.
+    Qed.
+
+    Lemma ISMin_intro : forall f,
+      IS R f -> exists g, IS (R @ supterm_eq) g /\ Min R g.
+
+    Proof.
+      intros f hf. set (Min' := fun f : nat -> NTM R =>
+        forall i x, subterm x (f i) -> forall g, g 0 = x -> ~IS R g).
+      cut (exists g : nat -> NTM R, IS S g /\ Min' g).
+      intros [g [h1 h2]]. exists (fun i => g i). intuition.
+      destruct (choice _ S_left_total) as [next hnext].
+      set (a := mkNTM (NT_min_term (NT_IS_elt 0 hf))).
+      exists (iter a next). split.
+      apply IS_iter. apply hnext.
+      unfold Min'. intros i x hx g g0 hg.
+      destruct (iter a next i) as [t [[h [h0 hh]] ht]].
+      simpl in hx. ded (ht _ hx). absurd (NT R x). hyp. exists g. intuition.
+    Qed.
+
+  End ISMin.
 
 End S.
